Lean4Lean/Theory/Typing.lean
@@ -4,14 +4,36 @@ namespace Lean4Lean
 
 open Lean (Name FVarId)
 
+inductive Ctx.LiftN (n : Nat) : Nat → List VExpr → List VExpr → Prop where
+  | zero : As.length = n → Ctx.LiftN n 0 Γ (As ++ Γ)
+  | succ : Ctx.LiftN n k Γ Γ' → Ctx.LiftN n (k+1) (A::Γ) (A.liftN n k :: Γ')
+
 inductive Lookup : List VExpr → Nat → VExpr → Prop where
   | zero : Lookup (ty::Γ) 0 ty.lift
-  | succ : Lookup Γ n ty → Lookup (ty::Γ) (n+1) ty.lift
+  | succ : Lookup Γ n ty → Lookup (A::Γ) (n+1) ty.lift
 
+theorem Lookup.lt (H : Lookup Γ i A) : i < Γ.length := by
+  induction H with
+  | zero => apply Nat.succ_pos
+  | succ _ ih => apply Nat.succ_lt_succ ih
+
+theorem Lookup.weakN (W : Ctx.LiftN n k Γ Γ') (H : Lookup Γ i A) :
+    Lookup Γ' (liftVar n i k) (A.liftN n k) := by
+  induction W generalizing i A with
+  | @zero Γ As =>
+    rw [liftVar_base]
+    subst n
+    induction As with simp [*, Nat.succ_add]
+    | cons _ _ ih => rw [VExpr.liftN_zero]; exact .succ ih
+  | @succ k _ _ _ _ ih =>
+    match H with
+    | .zero => rw [liftVar_zero, ← VExpr.lift_liftN']; exact .zero
+    | .succ H => rw [liftVar_succ, ← VExpr.lift_liftN']; exact (ih H).succ
+
+variable (uvars : Nat) {U : Nat}
 variable
   (constants : Name → Option (Option VConstant))
-  (IsDefEq : List VExpr → VExpr → VExpr → Prop)
-  (uvars : Nat) in
+  (IsDefEq : List VExpr → VExpr → VExpr → Prop) in
 inductive HasType1 : List VExpr → VExpr → VExpr → Prop where
   | bvar : Lookup Γ i ty → HasType1 Γ (.bvar i) ty
   | sort : l.WF uvars → HasType1 Γ (.sort l) (.sort (.succ l))
@@ -34,6 +56,31 @@ inductive HasType1 : List VExpr → VExpr → VExpr → Prop where
     HasType1 Γ (.forallE A B) (.sort (.imax u v))
   | defeq : IsDefEq Γ A B → HasType1 Γ e A → HasType1 Γ e B
 
+theorem HasType1.mono
+    {constants constants' : Name → Option (Option VConstant)}
+    {IsDefEq IsDefEq' : List VExpr → VExpr → VExpr → Prop}
+    (hconst : ∀ {n a}, constants n = some a → constants' n = some a)
+    (hdefeq : ∀ {Γ e1 e2}, IsDefEq Γ e1 e2 → IsDefEq' Γ e1 e2)
+    (H : HasType1 U constants IsDefEq Γ e A) :
+    HasType1 U constants' IsDefEq' Γ e A := by
+  induction H with
+  | bvar h => exact .bvar h
+  | sort h => exact .sort h
+  | const h1 h2 h3 => exact .const (hconst h1) h2 h3
+  | app _ _ ih1 ih2 => exact .app ih1 ih2
+  | lam _ _ ih1 ih2 => exact .lam ih1 ih2
+  | forallE _ _ ih1 ih2 => exact .forallE ih1 ih2
+  | defeq h1 _ ih2 => exact .defeq (hdefeq h1) ih2
+
+theorem HasType1.closedN (H : HasType1 U C DF Γ e B) : e.ClosedN Γ.length := by
+  induction H with
+  | bvar h => exact h.lt
+  | sort | const => trivial
+  | app _ _ ih1 ih2
+  | lam _ _ ih1 ih2
+  | forallE _ _ ih1 ih2 => exact ⟨ih1, ih2⟩
+  | defeq _ _ ih => exact ih
+
 variable
   (defeqs : VDefEq → Prop)
   (HasType : List VExpr → VExpr → VExpr → Prop) in
@@ -45,7 +92,8 @@ inductive IsDefEq1 : List VExpr → VExpr → VExpr → Prop where
   | trans :
     IsDefEq1 Γ e₁ e₂ → IsDefEq1 Γ e₂ e₃ → IsDefEq1 Γ e₁ e₃
   | sort :
-    l ≈ l' → IsDefEq1 Γ (.sort l) (.sort l')
+    l.WF uvars → l'.WF uvars → l ≈ l' →
+    IsDefEq1 Γ (.sort l) (.sort l')
   | app :
     HasType Γ f (.forallE A B) → HasType Γ f' (.forallE A B) → IsDefEq1 Γ f f' →
     HasType Γ a A → HasType Γ a' A → IsDefEq1 Γ a a' →
@@ -71,26 +119,250 @@ inductive IsDefEq1 : List VExpr → VExpr → VExpr → Prop where
     defeqs df →
     (∀ l ∈ ls, l.WF uvars) →
     ls.length = df.uvars →
-    IsDefEq1 [] (df.lhs.instL ls) (df.rhs.instL ls)
+    IsDefEq1 Γ (df.lhs.instL ls) (df.rhs.instL ls)
 
-variable (env : VEnv) (uvars : Nat) in
-def HasTypeN : Nat → List VExpr → VExpr → VExpr → Prop
-  | 0 => fun _ _ _ => False
-  | n+1 => HasType1 env.constants (IsDefEq1 env.defeqs (HasTypeN n)) uvars
+theorem IsDefEq1.mono
+    {defeqs defeqs' : VDefEq → Prop}
+    {HasType HasType' : List VExpr → VExpr → VExpr → Prop}
+    (hdefeq : ∀ {df}, defeqs df → defeqs' df)
+    (htype : ∀ {Γ e A}, HasType Γ e A → HasType' Γ e A)
+    (H : IsDefEq1 U defeqs HasType Γ e1 e2) :
+    IsDefEq1 U defeqs' HasType' Γ e1 e2 := by
+  induction H with
+  | refl h => exact .refl (htype h)
+  | symm _ ih => exact .symm ih
+  | trans _ _ ih1 ih2 => exact .trans ih1 ih2
+  | sort h1 h2 h3 => exact .sort h1 h2 h3
+  | app h11 h12 _ h21 h22 _ ih1 ih2 =>
+    exact .app (htype h11) (htype h12) ih1 (htype h21) (htype h22) ih2
+  | lam _ _ ih1 ih2 => exact .lam ih1 ih2
+  | forallE _ _ ih1 ih2 => exact .forallE ih1 ih2
+  | beta h1 h2 => exact .beta (htype h1) (htype h2)
+  | eta h1 => exact .eta (htype h1)
+  | proofIrrel h1 h2 h3 => exact .proofIrrel (htype h1) (htype h2) (htype h3)
+  | extra h1 h2 h3 => exact .extra (hdefeq h1) h2 h3
 
-def IsDefEqN (env : VEnv) (uvars : Nat) (n : Nat) : List VExpr → VExpr → VExpr → Prop :=
-  IsDefEq1 env.defeqs (HasTypeN env uvars n)
+-- theorem IsDefEq1.hasType (H : IsDefEq1 U DF (HasType1 U C DF') Γ e e') :
+--     (∃ A, HasType1 U C DF' Γ e A) ∧ (∃ A, HasType1 U C DF' Γ e' A) := by
+--   induction H with
+--   | refl h => exact ⟨⟨_, h⟩, _, h⟩
+--   | symm _ ih => exact ⟨ih.2, ih.1⟩
+--   | trans _ _ ih1 ih2 => exact ⟨ih1.1, ih2.2⟩
+--   | sort h1 h2 h3 => exact ⟨⟨_, .sort h1⟩, ⟨_, .sort h2⟩⟩
+--   | app h11 h12 _ h21 h22 _ ih1 ih2 => exact ⟨⟨_, .app h11 h21⟩, ⟨_, .app h12 h22⟩⟩
+--   | lam h1 h2 ih1 ih2 =>
+--     have ⟨⟨A11, h11⟩, ⟨A12, h12⟩⟩ := ih1
+--     have ⟨⟨A21, h21⟩, ⟨A22, h22⟩⟩ := ih2
+--     exact ⟨⟨_, .lam _ hA⟩, ⟨_, .lam h12 h22⟩⟩
+--   | forallE _ _ ih1 ih2 => exact .forallE ih1 ih2
+--   | beta h1 h2 => exact .beta (htype h1) (htype h2)
+--   | eta h1 => exact .eta (htype h1)
+--   | proofIrrel h1 h2 h3 => exact .proofIrrel (htype h1) (htype h2) (htype h3)
+--   | extra h1 h2 h3 => exact .extra (hdefeq h1) h2 h3
 
-def HasType (env : VEnv) (uvars : Nat) (Γ : List VExpr) (e A : VExpr) : Prop :=
-  ∃ n, HasTypeN env uvars n Γ e A
+def Typing := Nat → List VExpr → VExpr → VExpr → Prop
 
-def IsDefEq (env : VEnv) (uvars : Nat) (Γ : List VExpr) (e A : VExpr) : Prop :=
-  ∃ n, IsDefEqN env uvars n Γ e A
+def Typing.IsClosedN (T : Typing) : Prop :=
+  ∀ {u Γ e A}, T u Γ e A → e.ClosedN Γ.length
 
-def IsType (env : VEnv) (uvars : Nat) (Γ : List VExpr) (A : VExpr) : Prop :=
-  ∃ u, HasType env uvars Γ A (.sort u)
+def Typing.IsWeakN (T : Typing) : Prop :=
+  ∀ {u n k Γ Γ' e A}, Ctx.LiftN n k Γ Γ' → T u Γ e A → T u Γ' (e.liftN n k) (A.liftN n k)
 
-theorem HasType.type_isType (h : HasType E U Γ e A) : IsType E U Γ A := sorry
+def Typing.IsWeakN.weak (hT : IsWeakN T) : T U Γ e B → T U (A::Γ) e.lift B.lift :=
+  hT (.zero (As := [A]) rfl)
 
-theorem HasType.isDefEq_hasType (h : IsDefEq E U Γ e e') :
-    ∃ A, HasType E U Γ e A ∧ HasType E U Γ e' A := sorry
+def Typing.IsType (T : Typing) (U : Nat) (Γ : List VExpr) (A : VExpr) : Prop :=
+  ∃ u, T U Γ A (.sort u)
+
+theorem Typing.IsType.closedN (hT : T.IsClosedN) : IsType T U Γ A → A.ClosedN Γ.length
+  | ⟨_, h⟩ => hT h
+
+theorem Typing.IsType.weakN (hT : T.IsWeakN) (W : Ctx.LiftN n k Γ Γ') :
+    IsType T U Γ B → IsType T U Γ' (B.liftN n k)
+  | ⟨_, h⟩ => ⟨_, hT W h⟩
+
+theorem Typing.IsType.weak (hT : T.IsWeakN) : IsType T U Γ B → IsType T U (A::Γ) B.lift
+  | ⟨_, h⟩ => ⟨_, hT (.zero (As := [A]) rfl) h⟩
+
+def VConstant.WF (T : Typing) (ci : VConstant) : Prop := T.IsType ci.uvars [] ci.type
+
+def VDefEq.WF (T : Typing) (df : VDefEq) : Prop :=
+  ∃ A, T df.uvars [] df.lhs A ∧ T df.uvars [] df.rhs A
+
+structure VPreEnv where
+  env : VEnv
+  protected T : Typing
+
+def VPreEnv.HasTypeN (P : VPreEnv) : Nat → Typing
+  | 0 => P.T
+  | n+1 => fun U Γ e A =>
+    P.HasTypeN n U Γ e A ∨
+    HasType1 U P.env.constants (IsDefEq1 U P.env.defeqs (P.HasTypeN n U)) Γ e A
+
+structure VPreEnv.LE (P1 P2 : VPreEnv) : Prop where
+  env : P1.env ≤ P2.env
+  T : P1.T u Γ e A → P2.T u Γ e A
+
+instance : LE VPreEnv := ⟨VPreEnv.LE⟩
+
+theorem VPreEnv.le_refl (env : VPreEnv) : env ≤ env := ⟨VEnv.le_refl _, id⟩
+
+theorem VPreEnv.le_trans {a b c : VPreEnv} (h1 : a ≤ b) (h2 : b ≤ c) : a ≤ c :=
+  ⟨VEnv.le_trans h1.1 h2.1, h2.2 ∘ h1.2⟩
+
+namespace VPreEnv
+variable (P : VPreEnv)
+
+theorem HasTypeN.mono {P P' : VPreEnv} {n n' : Nat} (hP : P ≤ P') (hn : n ≤ n')
+    (H : P.HasTypeN n U Γ e A) : P'.HasTypeN n' U Γ e A :=
+  match n, n', hn with
+  | 0, 0, _ => hP.2 H
+  | 0, _+1, _ => Or.inl <| HasTypeN.mono hP (Nat.zero_le _) H
+  | _+1, _+1, hn =>
+    have IH := fun {Γ e A} =>
+      HasTypeN.mono hP (Nat.le_of_succ_le_succ hn) (Γ := Γ) (e := e) (A := A)
+    Or.imp IH (HasType1.mono @hP.1.1 (IsDefEq1.mono @hP.1.2 IH)) H
+
+def IsDefEqN (n U : Nat) : List VExpr → VExpr → VExpr → Prop :=
+  IsDefEq1 U P.env.defeqs (P.HasTypeN n U)
+
+theorem IsDefEqN.mono {P P' : VPreEnv} {n n' : Nat} (hP : P ≤ P') (hn : n ≤ n') :
+    P.IsDefEqN n U Γ e A → P'.IsDefEqN n' U Γ e A :=
+  IsDefEq1.mono @hP.1.2 (HasTypeN.mono hP hn)
+
+def HasType : Typing := fun U Γ e A => ∃ n, P.HasTypeN U n Γ e A
+
+theorem HasType.mono {P P' : VPreEnv} (hP : P ≤ P') : P.HasType U Γ e A → P'.HasType U Γ e A
+  | ⟨n, h⟩ => ⟨n, h.mono hP (Nat.le_refl _)⟩
+
+def IsDefEq (P : VPreEnv) (U : Nat) (Γ : List VExpr) (e A : VExpr) : Prop :=
+  ∃ n, P.IsDefEqN n U Γ e A
+
+theorem IsDefEq.mono {P P' : VPreEnv} (hP : P ≤ P') : P.IsDefEq U Γ e A → P'.IsDefEq U Γ e A
+  | ⟨n, h⟩ => ⟨n, h.mono hP (Nat.le_refl _)⟩
+
+def IsType (P : VPreEnv) := P.HasType.IsType
+
+theorem IsType.mono {P P' : VPreEnv} (hP : P ≤ P') : P.IsType U Γ A → P'.IsType U Γ A
+  | ⟨u, h⟩ => ⟨u, h.mono hP⟩
+
+end VPreEnv
+
+structure VPreEnvWF extends VPreEnv where
+  closedN : T.IsClosedN
+  weakN : T.IsWeakN
+  constWF : env.constants n = some (some ci) → ci.WF T
+  defeqWF : env.defeqs df → df.WF T
+
+instance : LE VPreEnvWF := ⟨(·.toVPreEnv ≤ ·.toVPreEnv)⟩
+
+variable {P : VPreEnvWF}
+
+namespace VPreEnv
+
+theorem HasTypeN.closedN {P : VPreEnvWF} : ∀ {n}, P.HasTypeN n U Γ e B → e.ClosedN Γ.length
+  | 0, h => P.closedN h
+  | _+1, .inl h => HasTypeN.closedN h
+  | _+1, .inr h => HasType1.closedN h
+
+theorem HasType.closedN : P.HasType.IsClosedN
+  | _, _, _, _, ⟨_, h⟩ => h.closedN
+
+theorem IsType.closedN : P.IsType U Γ A → A.ClosedN Γ.length :=
+  Typing.IsType.closedN HasType.closedN
+
+end VPreEnv
+
+variable
+  {C : Name → Option (Option VConstant)}
+  {DF : List VExpr → VExpr → VExpr → Prop}
+  (closedN : T.IsClosedN)
+  (hconst : ∀ {n ci}, C n = some (some ci) → ci.WF T)
+  (hdefeq : ∀ {n k Γ Γ' A B}, Ctx.LiftN n k Γ Γ' → DF Γ A B → DF Γ' (A.liftN n k) (B.liftN n k)) in
+theorem HasType1.weakN
+    (W : Ctx.LiftN n k Γ Γ')
+    (H : HasType1 U C DF Γ e B) :
+    HasType1 U C DF Γ' (e.liftN n k) (B.liftN n k) := by
+  induction H generalizing k Γ' with
+  | bvar h => refine .bvar (h.weakN W)
+  | sort h => exact .sort h
+  | const h1 h2 h3 =>
+    rw [((hconst h1).closedN closedN).instL.liftN_eq (Nat.zero_le _)]
+    exact .const h1 h2 h3
+  | app _ _ ih1 ih2 => exact (by simpa using VExpr.liftN_inst_hi ..) ▸ .app (ih1 W) (ih2 W)
+  | lam _ _ ih1 ih2 => exact .lam (ih1 W) (ih2 W.succ)
+  | forallE _ _ ih1 ih2 => exact .forallE (ih1 W) (ih2 W.succ)
+  | defeq h1 _ ih2 => exact .defeq (hdefeq W h1) (ih2 W)
+
+variable
+  {DF : VDefEq → Prop}
+  {TY : List VExpr → VExpr → VExpr → Prop}
+  (closedN : T.IsClosedN)
+  (hdefeq : ∀ {df}, DF df → df.WF T)
+  (htype : ∀ {n k Γ Γ' e A}, Ctx.LiftN n k Γ Γ' → TY Γ e A → TY Γ' (e.liftN n k) (A.liftN n k)) in
+theorem IsDefEq1.weakN (W : Ctx.LiftN n k Γ Γ') (H : IsDefEq1 U DF TY Γ e1 e2) :
+    IsDefEq1 U DF TY Γ' (e1.liftN n k) (e2.liftN n k) := by
+  induction H generalizing k Γ' with
+  | refl h => exact .refl (htype W h)
+  | symm _ ih => exact .symm (ih W)
+  | trans _ _ ih1 ih2 => exact .trans (ih1 W) (ih2 W)
+  | sort h1 h2 h3 => exact .sort h1 h2 h3
+  | app h11 h12 _ h21 h22 _ ih1 ih2 =>
+    exact .app (htype W h11) (htype W h12) (ih1 W) (htype W h21) (htype W h22) (ih2 W)
+  | lam _ _ ih1 ih2 => exact .lam (ih1 W) (ih2 W.succ)
+  | forallE _ _ ih1 ih2 => exact .forallE (ih1 W) (ih2 W.succ)
+  | beta h1 h2 =>
+    exact (by simpa using VExpr.liftN_inst_hi ..) ▸ .beta (htype W.succ h1) (htype W h2)
+  | eta h1 =>
+    have := IsDefEq1.eta (uvars := U) (defeqs := DF) (htype W h1)
+    simp [VExpr.liftN]; rwa [VExpr.liftN_zero, ← VExpr.lift_liftN']
+  | proofIrrel h1 h2 h3 => exact .proofIrrel (htype W h1) (htype W h2) (htype W h3)
+  | extra h1 h2 h3 =>
+    have ⟨A, hA1, hA2⟩ := hdefeq h1
+    rw [(closedN hA1).instL.liftN_eq (Nat.zero_le _), (closedN hA2).instL.liftN_eq (Nat.zero_le _)]
+    exact .extra h1 h2 h3
+
+namespace VPreEnv
+
+theorem HasTypeN.weakN : ∀ {n}, (P.HasTypeN n).IsWeakN
+  | 0 => P.weakN
+  | _+1 => fun
+    | W, .inl h => .inl <| HasTypeN.weakN W h
+    | W, .inr h => .inr <| HasType1.weakN P.closedN P.constWF
+      (IsDefEq1.weakN P.closedN P.defeqWF HasTypeN.weakN) W h
+
+theorem IsDefEqN.weakN (W : Ctx.LiftN n k Γ Γ')
+    (h : P.IsDefEqN U N Γ e1 e2) : P.IsDefEqN U N Γ' (e1.liftN n k) (e2.liftN n k) :=
+  IsDefEq1.weakN P.closedN P.defeqWF HasTypeN.weakN W h
+
+theorem HasType.weakN : P.HasType.IsWeakN := fun W ⟨_, h⟩ => ⟨_, h.weakN W⟩
+
+theorem IsType.weakN (W : Ctx.LiftN n k Γ Γ') : P.IsType U Γ B → P.IsType U Γ' (B.liftN n k)
+  | ⟨_, h⟩ => ⟨_, h.weakN W⟩
+
+end VPreEnv
+
+def Typing.CtxWF (T : Typing) (Γ : List VExpr) : Prop := ∀ {n A}, Lookup Γ n A → T.IsType uvars Γ A
+
+def Typing.CtxWF.zero {T : Typing} : T.CtxWF U [] := fun.
+
+def Typing.CtxWF.succ {T : Typing} (hT : T.IsWeakN)
+    (H : T.CtxWF U Γ) (hA : T.IsType U Γ A) : T.CtxWF U (A::Γ)
+  | _, _, .zero => hA.weak hT
+  | _, _, .succ h => (H h).weak hT
+
+-- theorem HasType.type_isType {T : Typing} (hΓ : T.CtxWF U Γ)
+--     (H : HasType1 U C DF Γ e A) : ∃ u, HasType1 U C DF Γ A (.sort u) := by
+--   induction H with
+--   | bvar h => exact hΓ h
+--   | sort h => exact ⟨_, n+1, .sort h⟩
+--   | const h1 h2 h3 =>
+--     have := henv.1 h1
+--     exact _
+--   | app _ _ ih1 ih2 => exact .app ih1 ih2
+--   | lam _ _ ih1 ih2 => exact .lam ih1 ih2
+--   | forallE _ _ ih1 ih2 => exact .forallE ih1 ih2
+--   | defeq h1 _ ih2 => exact .defeq (hdefeq h1) ih2
+
+-- theorem IsDefEq.hasType (h : IsDefEq U E Γ e e') :
+--     ∃ A, HasType U E Γ e A ∧ HasType U E Γ e' A := sorry
