Lean4Lean/Std/Logic.lean
@@ -1,3 +1,7 @@
+import Std.Data.Nat.Lemmas
 
 theorem funext_iff {β : α → Sort u} {f₁ f₂ : ∀ x : α, β x} : f₁ = f₂ ↔ ∀ a, f₁ a = f₂ a :=
   Iff.intro (fun h _ ↦ h ▸ rfl) funext
+
+protected theorem Nat.lt_add_left (a b c : Nat) (h : a < c) : a < b + c :=
+  Nat.add_comm .. ▸ Nat.lt_add_right _ _ _ h
